{
 "cells": [
  {
   "cell_type": "markdown",
   "metadata": {},
   "source": [
    "# Constant-Coefficient Homogeneus Linear Second-Order ODE - Theory\n",
    "\n",
    "An constant-coefficient homogeneus linear second-order ODE has the following format:\n",
    "$$\\frac{d^2y}{dx}+p\\frac{dy}{dx}+qy(x) = 0$$\n",
    "where $p,q \\in \\mathbb{R}$.\n",
    "\n",
    "## The Equation's Solution\n",
    "The general solution $y(x)$ for this type of equation is a linear combination of two fundamental solutions $y_1(x)$ and $y_1(x)$:\n",
    "\n",
    "$$y(x) = c_1y_1(x) + c_2y_2(x)$$\n",
    "\n",
    "where $c_1$ and $c_2$ are constants that must be found by solving de initial value problem.\n",
    "\n",
    "In general, for this type of ODE, the fundamental solutions have the following format:\n",
    "$$y(x) = e^{\\lambda x}$$\n",
    "where $\\lambda_n \\in \\mathbb{C}$.\n",
    "\n",
    "### Characteristic Equation\n",
    "\n",
    "To find the $\\lambda$ for each of the two fundamental solutions, it is necessary to solve the following characteristic quadratic equation:\n",
    "\n",
    "$$\\lambda^2 e^{\\lambda x} + p \\lambda e^{\\lambda x} + q e^{\\lambda x} = 0$$\n",
    "\n",
    "which is equivalent to\n",
    "\n",
    "$$e^{\\lambda x} (\\lambda^2 + p \\lambda + q ) = 0$$\n",
    "\n",
    "It is a fact that $\\not \\exists t \\in \\mathbb{C}: e^t = 0$, therefore:\n",
    "\n",
    "$$\\lambda^2 + p \\lambda + q = 0$$\n",
    "\n",
    "Applying the quadratic formula, we have:\n",
    "\n",
    "$$\\lambda_1 = \\frac{-p + \\sqrt{\\Delta}}{2}$$\n",
    "$$\\lambda_2 = \\frac{-p - \\sqrt{\\Delta}}{2}$$\n",
    "\n",
    "where $\\Delta = p^2 - 4q$.\n",
    "\n",
    "### Fundamental and General Solutions\n",
    "The fundamental solutions $y_1(x)$ and $y_2(x)$ need to be linearly independent. This linear independence can be verified by the Wronskian. The characteristc equation can have two real roots, one real root or two complex roots, and there are a pair of fundamentally linearly independent solutions for each of these cases.\n",
    "\n",
    "#### Case $\\Delta > 0$\n",
    "\n",
    "In this case, $\\lambda_1, \\lambda_2 \\in \\mathbb{R}$ and $\\lambda_1 \\neq \\lambda_2$.\n",
    "\n",
    "The fundamental solutions are:\n",
    "\n",
    "$$y_1(x)=e^{\\lambda_1 x}$$\n",
    "\n",
    "$$y_2(x)=e^{\\lambda_2 x}$$\n",
    "\n",
    "The general solution is:\n",
    "\n",
    "$$y(x) = c_1 e^{\\lambda_1 x} + c_2 e^{\\lambda_2 x}$$\n",
    "\n",
    "where $c_1, c_2 \\in \\mathbb{R}$.\n",
    "\n",
    "#### Case $\\Delta = 0$\n",
    "\n",
    "In this case, $\\lambda = \\lambda_1 = \\lambda_2$ and $\\lambda \\in \\mathbb{R}$.\n",
    "\n",
    "The fundamental solutions are:\n",
    "\n",
    "$$y_1(x)= e^{\\lambda x}$$\n",
    "\n",
    "$$y_2(x)= x e^{\\lambda x}$$\n",
    "\n",
    "The general solution is:\n",
    "\n",
    "$$y(x) = c_1 e^{\\lambda x} + c_2 x e^{\\lambda x}$$\n",
    "\n",
    "where $c_1, c_2 \\in \\mathbb{R}$.\n",
    "\n",
    "#### Case $\\Delta < 0$\n",
    "\n",
    "In this case, $\\lambda_1, \\lambda_2 \\in \\mathbb{C}$. These roots are:\n",
    "\n",
    "$$\\lambda_1 = \\alpha + \\beta i$$\n",
    "$$\\lambda_2 = \\alpha - \\beta i$$\n",
    "\n",
    "The fundamental solutions are:\n",
    "\n",
    "$$y_1(x) = e^{\\lambda_1 x} = e^{x(\\alpha + \\beta i)} = e^{x \\alpha } e^{x \\beta i}$$\n",
    "\n",
    "$$y_2(x) = e^{\\lambda_2 x} = e^{x(\\alpha - \\beta i)} = e^{x \\alpha } e^{-x \\beta i}$$\n",
    "\n",
    "By applying the Euler's indentity ($e^{i\\theta} = \\cos\\theta + i\\sin\\theta$), we find out:\n",
    "\n",
    "$$y_1(x) = e^{x \\alpha } e^{x \\beta i} = e^{x \\alpha } [\\cos(\\beta x) + i\\sin(\\beta x)]$$\n",
    "\n",
    "$$y_2(x) = e^{x \\alpha } e^{-x \\beta i} = e^{x \\alpha } [\\cos(\\beta x) - i\\sin(\\beta x)] $$\n",
    "\n",
    "The general solution is therefore:\n",
    "\n",
    "$$y(x) = c_1 e^{\\lambda_1 x} + c_2 e^{\\lambda_2 x} = c_1 e^{x \\alpha } [\\cos(\\beta x) + i\\sin(\\beta x)] + c_2 e^{x \\alpha } [\\cos(\\beta x) - i\\sin(\\beta x)]$$\n",
    "\n",
    "$$ = e^{x \\alpha } [\\cos(\\beta x)(c_1 + c_2) + i\\sin(\\beta x)(c_1 - c_2)]$$\n",
    "\n",
    "where $c_1, c_2 \\in \\mathbb{R}$. \n",
    "\n",
    "Considering $k_1 = (c_1 + c_2)$ and $k_2 = i(c_1 - c_2)$, we have:\n",
    "\n",
    "$$y(x) = e^{x \\alpha } [k_1\\cos(\\beta x) + k_2\\sin(\\beta x)]$$"
   ]
  },
  {
   "cell_type": "markdown",
   "metadata": {},
   "source": [
    "# Practice with Python\n",
    "\n",
    "TODO"
   ]
  },
  {
   "cell_type": "code",
   "execution_count": null,
   "metadata": {},
   "outputs": [],
   "source": []
  }
 ],
 "metadata": {
  "kernelspec": {
   "display_name": "Python 3",
   "language": "python",
   "name": "python3"
  },
  "language_info": {
   "codemirror_mode": {
    "name": "ipython",
    "version": 3
   },
   "file_extension": ".py",
   "mimetype": "text/x-python",
   "name": "python",
   "nbconvert_exporter": "python",
   "pygments_lexer": "ipython3",
   "version": "3.7.6"
  }
 },
 "nbformat": 4,
 "nbformat_minor": 4
}
